cancel_sound, with one admit about pure subformulas

platform/Depl/Cancel.v
@@ -28,6 +28,21 @@ Hint Rewrite fos_set_eq fos_set_ne using congruence.
 
 (** * Local proof automation *)
 
+Theorem fo_set_eq : forall fE x e,
+  fo_set fE x e x = e.
+Proof.
+  unfold fo_set; intros; destruct (string_dec x x); tauto.
+Qed.
+
+Theorem fo_set_ne : forall fE x e y,
+  y <> x
+  -> fo_set fE x e y = fE y.
+Proof.
+  unfold fo_set; intros; destruct (string_dec y x); tauto.
+Qed.
+
+Hint Rewrite fo_set_eq fo_set_ne using congruence.
+
 Inductive notThisOne := NotThisOne.
 
 Ltac t := simpl; intuition;
@@ -196,14 +211,20 @@ Definition unify_expr (s : fo_sub) (lhs rhs : expr)
     | _, _ => None
   end.
 
-Theorem unify_expr_sound : forall fE s lhs rhs s' fs,
+Theorem unify_expr_sound : forall fE s s'' lhs rhs s' fs,
   unify_expr s lhs rhs = Some (s', fs)
-  -> List.Forall (fun f : _ -> _ -> Prop =>
-    forall s'', (forall x v, s'' x = Some v -> s' x = Some v) -> f fE s'') fs
-  -> exists rhs', sub_expr s' rhs = Some rhs'
+  -> List.Forall (fun f => f fE s'') fs
+  -> (forall x v, s' x = Some v -> s'' x = Some v)
+  -> exists rhs', sub_expr s'' rhs = Some rhs'
     /\ exprD lhs fE = exprD rhs' fE.
 Proof.
   destruct lhs, rhs; t.
+  repeat esplit.
+  apply H1; t.
+  t.
+  repeat esplit.
+  apply H1; t.
+  t.
 Qed.
 
 Theorem unify_expr_monotone : forall s lhs rhs s' fs,
@@ -244,25 +265,13 @@ Qed.
 
 Local Hint Immediate map_nil map_cons.
 
-Ltac unify_args := t;
-  match goal with
-    | [ _ : context[unify_args ?s ?lhs ?rhs], IH : forall rhs : list expr, _ |- _ ] =>
-      let Heq := fresh in
-      specialize (IH rhs s); case_eq (unify_args s lhs rhs); [
-        intros ? Heq; rewrite Heq in *;
-          match goal with
-            | [ p : prod _ _ |- _ ] => destruct p
-          end; specialize (IH _ _ eq_refl)
-        | intro Heq; rewrite Heq in *; discriminate ]
-  end; t.
-
 Local Hint Resolve unify_expr_monotone.
 
 Theorem unify_args_monotone : forall lhs rhs s s' fs,
   unify_args s lhs rhs = Some (s', fs)
   -> forall x e, s x = Some e -> s' x = Some e.
 Proof.
-  induction lhs; destruct rhs; unify_args.
+  induction lhs; destruct rhs; t.
 Qed.
 
 Local Hint Resolve unify_args_monotone.
@@ -281,55 +290,43 @@ Proof.
   induction ls1; simpl; try solve [ eauto ]; inversion_clear 1; eauto.
 Qed.
 
-Theorem unify_args_sound : forall fE lhs rhs s s' fs,
+Local Hint Immediate Forall_app_fwd1 Forall_app_fwd2.
+
+Theorem unify_args_sound : forall fE s'' lhs rhs s s' fs,
   unify_args s lhs rhs = Some (s', fs)
-  -> List.Forall (fun f : _ -> _ -> Prop =>
-    forall s'', (forall x v, s'' x = Some v -> s' x = Some v) -> f fE s'') fs
-  -> exists rhs', sub_exprs s' rhs = Some rhs'
+  -> List.Forall (fun f => f fE s'') fs
+  -> (forall x v, s' x = Some v -> s'' x = Some v)
+  -> exists rhs', sub_exprs s'' rhs = Some rhs'
     /\ map (fun e => exprD e fE) lhs = map (fun e => exprD e fE) rhs'.
 Proof.
-  induction lhs; destruct rhs; unify_args;
-    match goal with
-      | [ H : _ |- _ ] => specialize (unify_expr_sound fE _ _ _ _ _ H); t
-    end;
-    repeat esplit; eauto.
-  specialize (Forall_app_fwd1 _ _ _ _ H0).
-  specialize (Forall_app_fwd2 _ _ _ _ H0).
-  t.
-  destruct H2.
-  eapply Forall_weaken; [ | eassumption ]; eauto.
-  t.
-  edestruct sub_expr_monotone.
-  Focus 4.
-  destruct H2.
-  rewrite H2.
-
+  induction lhs; destruct rhs; t.
+  edestruct unify_expr_sound; eauto; t.
+  edestruct IHlhs; eauto; t.
 Qed.
 
-Definition unify_pred (s : fo_sub) (lhs rhs : pred) : option (fo_sub * list Prop) :=
+Definition unify_pred (s : fo_sub) (lhs rhs : pred) : option (fo_sub * list (fo_env -> fo_sub -> Prop)) :=
   match lhs, rhs with
     | Named X1 es1, Named X2 es2 =>
       if string_dec X1 X2 then unify_args s es1 es2 else None
     | _, _ => None
   end.
 
-Theorem unify_pred_monotone : forall lhs rhs s s' Ps,
-  unify_pred s lhs rhs = Some (s', Ps)
+Theorem unify_pred_monotone : forall lhs rhs s s' fs,
+  unify_pred s lhs rhs = Some (s', fs)
   -> forall x e, s x = Some e -> s' x = Some e.
 Proof.
-  destruct lhs, rhs; unify_args.
+  destruct lhs, rhs; t.
 Qed.
 
-Theorem unify_pred_sound : forall G (hE : ho_env G) fE lhs rhs s s' Ps,
-  unify_pred s lhs rhs = Some (s', Ps)
-  -> vcs Ps
-  -> exists rhs', sub_pred s' rhs = Some rhs'
+Theorem unify_pred_sound : forall G (hE : ho_env G) fE s'' lhs rhs s s' fs,
+  unify_pred s lhs rhs = Some (s', fs)
+  -> List.Forall (fun f => f fE s'') fs
+  -> (forall x v, s' x = Some v -> s'' x = Some v)
+  -> exists rhs', sub_pred s'' rhs = Some rhs'
     /\ predD lhs hE fE = predD rhs' hE fE.
 Proof.
-  destruct lhs, rhs; t;
-    match goal with
-      | [ H : _ |- _ ] => specialize (unify_args_sound fE _ _ _ _ _ H); t
-    end.
+  destruct lhs, rhs; t.
+  edestruct unify_args_sound; eauto; t.
 Qed.
 
 
@@ -337,12 +334,13 @@ Qed.
 
 (** Result of cancelation *)
 Inductive result :=
-| Success (NewLhs : list pred) (ProveThese : list Prop)
+| Success (NewLhs : list pred) (ProveThis : Prop)
 | Failure (Message : Prop).
 
 (** Result of canceling just one atomic predicate *)
 Inductive result1 :=
-| Success1 (NewSub : fo_sub) (NewLhs : list pred) (ProveThese : list Prop)
+| Success1 (NewSub : fo_sub) (NewLhs : list pred)
+  (ProveThese : list (fo_env -> fo_sub -> Prop))
 | Failure1 (Message : Prop).
 
 Inductive noMatchFor (rhs : pred) := .
@@ -353,10 +351,10 @@ Fixpoint findMatching (s : fo_sub) (lhs : list pred) (rhs : pred) : result1 :=
     | nil => Failure1 (noMatchFor rhs)
     | p :: lhs =>
       match unify_pred s p rhs with
-        | Some (s, Ps) => Success1 s lhs Ps 
+        | Some (s, fs) => Success1 s lhs fs
         | None =>
           match findMatching s lhs rhs with
-            | Success1 s lhs Ps => Success1 s (p :: lhs) Ps
+            | Success1 s lhs fs => Success1 s (p :: lhs) fs
             | x => x
           end
       end
@@ -364,8 +362,8 @@ Fixpoint findMatching (s : fo_sub) (lhs : list pred) (rhs : pred) : result1 :=
 
 Local Hint Resolve unify_pred_monotone.
 
-Theorem findMatching_monotone : forall rhs lhs s s' lhs' Ps,
-  findMatching s lhs rhs = Success1 s' lhs' Ps
+Theorem findMatching_monotone : forall rhs lhs s s' lhs' fs,
+  findMatching s lhs rhs = Success1 s' lhs' fs
   -> forall x e, s x = Some e -> s' x = Some e.
 Proof.
   induction lhs; t.
@@ -379,10 +377,11 @@ Qed.
 
 Local Hint Resolve findMatching_monotone.
 
-Theorem findMatching_sound : forall G (hE : ho_env G) S fE rhs lhs s s' lhs' Ps,
-  findMatching s lhs rhs = Success1 s' lhs' Ps
-  -> vcs Ps
-  -> exists rhs', sub_pred s' rhs = Some rhs'
+Theorem findMatching_sound : forall G (hE : ho_env G) S fE rhs s'' lhs s s' lhs' fs,
+  findMatching s lhs rhs = Success1 s' lhs' fs
+  -> List.Forall (fun f => f fE s'') fs
+  -> (forall x v, s' x = Some v -> s'' x = Some v)
+  -> exists rhs', sub_pred s'' rhs = Some rhs'
     /\ (SubstsH S (fold_left (fun hp p => starB (predD p hE fE) hp) lhs (empB _))
     ===> SubstsH S (predD rhs' hE fE)
     * SubstsH S (fold_left (fun hp p => starB (predD p hE fE) hp) lhs' (empB _))).
@@ -392,7 +391,7 @@ Proof.
   match goal with
     | [ H : Success1 _ _ _ = Success1 _ _ _ |- _ ] => injection H; clear H; intros; subst
   end.
-  eapply unify_pred_sound in H1; eauto; t.
+  edestruct unify_pred_sound; eauto; t.
   repeat esplit.
   eapply Himp_trans; [ apply star_out_fwd | ].
   apply SubstsH_star_fwd.
@@ -425,17 +424,17 @@ Fixpoint findMatchings (s : fo_sub) (lhs rhs : list pred) : result1 :=
     | nil => Success1 s lhs nil
     | p :: rhs =>
       match findMatching s lhs p with
-        | Success1 s lhs Ps =>
+        | Success1 s lhs fs =>
           match findMatchings s lhs rhs with
-            | Success1 s lhs Ps' => Success1 s lhs (Ps ++ Ps')
+            | Success1 s lhs fs' => Success1 s lhs (fs ++ fs')
             | x => x
           end
         | x => x
       end
   end.
 
-Theorem findMatchings_monotone : forall rhs lhs s s' lhs' Ps,
-  findMatchings s lhs rhs = Success1 s' lhs' Ps
+Theorem findMatchings_monotone : forall rhs lhs s s' lhs' fs,
+  findMatchings s lhs rhs = Success1 s' lhs' fs
   -> forall x e, s x = Some e -> s' x = Some e.
 Proof.
   induction rhs; t.
@@ -452,10 +451,11 @@ Qed.
 
 Local Hint Resolve findMatchings_monotone.
 
-Theorem findMatchings_sound : forall G (hE : ho_env G) S fE rhs lhs s s' lhs' Ps,
-  findMatchings s lhs rhs = Success1 s' lhs' Ps
-  -> vcs Ps
-  -> exists rhs', sub_preds s' rhs = Some rhs'
+Theorem findMatchings_sound : forall G (hE : ho_env G) S fE rhs s'' lhs s s' lhs' fs,
+  findMatchings s lhs rhs = Success1 s' lhs' fs
+  -> List.Forall (fun f => f fE s'') fs
+  -> (forall x v, s' x = Some v -> s'' x = Some v)
+  -> exists rhs', sub_preds s'' rhs = Some rhs'
     /\ (SubstsH S (fold_left (fun hp p => starB (predD p hE fE) hp) lhs (empB _))
     ===> SubstsH S (fold_left (fun hp p => starB (predD p hE fE) hp) rhs' (empB _))
     * SubstsH S (fold_left (fun hp p => starB (predD p hE fE) hp) lhs' (empB _))).
@@ -473,18 +473,18 @@ Proof.
         rewrite Heq in *; try discriminate
   end.
   match goal with
-    | [ _ : context[findMatchings ?s ?lhs ?rhs], IH : forall lhs : list pred, _ |- _ ] =>
-      let Heq := fresh in specialize (IH lhs s); case_eq (findMatchings s lhs rhs);
+    | [ _ : context[findMatchings ?s ?lhs ?rhs], IH : forall s'' : fo_sub, _ |- _ ] =>
+      let Heq := fresh in specialize (IH s'' lhs s); case_eq (findMatchings s lhs rhs);
         [ intros ? ? ? Heq; rewrite Heq in *; specialize (IH _ _ _ eq_refl)
           | intros ? Heq; rewrite Heq in *; try discriminate ]
   end.
   match goal with
     | [ H : Success1 _ _ _ = Success1 _ _ _ |- _ ] => injection H; clear H; intros; subst
   end; t.
-  specialize (findMatching_sound _ hE S fE _ _ _ _ _ _ H1); t.
-  erewrite sub_pred_monotone; [ .. | eauto ]; eauto.
+  edestruct findMatching_sound; eauto; t.
+  edestruct IHrhs; eauto; t.
   repeat esplit.
-  eapply Himp_trans; [ apply H6 | ].
+  eapply Himp_trans; [ apply H5 | ].
   simpl.
   eapply Himp_trans; [ | apply Himp_star_frame; [ apply star_out_bwd | apply Himp_refl ] ].
   eapply Himp_trans; [ | apply Himp_star_frame; [ apply SubstsH_star_bwd | apply Himp_refl ] ].
@@ -492,18 +492,19 @@ Proof.
   apply Himp_star_frame; auto; apply Himp_refl.
 Qed.
 
-(** Overall cancelation *)
+(** Overall cancellation *)
 Definition cancel (lhs rhs : normal) : result :=
   match findMatchings fos_empty (NImpure lhs) (NImpure rhs) with
     | Failure1 msg => Failure msg
-    | Success1 s lhs' Ps => Success lhs' (
+    | Success1 s lhs' fs => Success lhs' (
       (forall x, In x (NQuants rhs) -> s x <> None)
-      :: match NPure rhs with
-           | None => Ps
+      /\ (forall fE, List.Forall (fun f => f fE s) fs)
+      /\ match NPure rhs with
+           | None => True
            | Some P =>
              (forall fE1 fE2, (forall x, s x <> None -> fE1 x = fE2 x)
                -> P fE1 = P fE2)
-             :: (forall fE,
+             /\ (forall fE,
                let fE' := (fun x => match s x with
                                       | None => Dyn tt
                                       | Some e => exprD e fE
@@ -512,13 +513,13 @@ Definition cancel (lhs rhs : normal) : result :=
                  | None => P fE'
                  | Some P1 => P1 fE -> P fE'
                end)
-             :: Ps
          end)
   end.
 
-Theorem cancel_sound : forall fE G (hE : ho_env G) S lhs rhs lhs' Ps,
-  cancel lhs rhs = Success lhs' Ps
-  -> vcs Ps
+Theorem cancel_sound : forall fE G (hE : ho_env G) S lhs rhs lhs' P,
+  cancel lhs rhs = Success lhs' P
+  -> P
+  -> List.Forall (wellScoped (NQuants rhs)) (NImpure rhs)
   -> SubstsH S (normalD lhs hE fE)
   ===> SubstsH S (normalD rhs hE fE)
   * SubstsH S (normalD {| NQuants := NQuants lhs;
@@ -529,13 +530,11 @@ Proof.
   
   case_eq (findMatchings fos_empty (NImpure lhs) (NImpure rhs)); intros.
   Focus 2.
-  rewrite H1 in *; discriminate.
+  rewrite H2 in *; discriminate.
 
-  rewrite H1 in *.
-  injection H; clear H; intros; subst.
-  inversion H0; clear H0; intros; subst.
-  assert (vcs ProveThese) by t.
-  specialize (fun fE => findMatchings_sound _ hE S fE _ _ _ _ _ _ H1); intro Hfms.
+  rewrite H2 in *.
+  injection H; clear H; intros; subst; intuition.
+
   eapply Himp_trans; [ | apply Himp_star_comm ].
 
   Lemma addQuants_gulp : forall G (f : _ -> hpropB G) S p qs fE,
@@ -558,8 +557,7 @@ Proof.
   eapply Himp_trans; [ | apply addQuants_gulp ].
   simpl.
   apply addQuants_monotone; intros.
-  specialize (Hfms fE'); intuition.
-  destruct H2; intuition.
+  edestruct findMatchings_sound; eauto; intuition.
   eapply Himp_trans; [ apply multistar_weaken | ].
   instantiate (1 := (match NPure lhs with
                        | Some P => [|P fE'|]
@@ -571,183 +569,315 @@ Proof.
   apply Himp_star_Emp'.
   eapply Himp_trans; [ apply star_out_fwd | ].
   eapply Himp_trans; [ apply SubstsH_star_fwd | ].
-  eapply Himp_trans; [ apply Himp_star_frame; [ apply Himp_refl | apply H6 ] | ].
+  eapply Himp_trans; [ apply Himp_star_frame; [ apply Himp_refl | apply H7 ] | ].
   eapply Himp_trans; [ | apply SubstsH_star_bwd ].
   eapply Himp_trans; [ apply Himp_star_assoc' | ].
   eapply Himp_trans; [ apply Himp_star_comm | ].
   apply Himp_star_frame; try apply Himp_refl.
-  
-  Lemma sub_expr_closed : forall s e,
-    (forall fE fE', exprD e fE = exprD e fE')
-    -> forall e', sub_expr s e = Some e'
-      -> e' = e.
+  clear H7.
+
+  unfold normalD.
+  eapply Himp_trans; [ apply Himp_star_frame; [ | apply Himp_refl ] | ].
+  instantiate (1 := [| match NPure lhs with
+                         | Some P => P fE'
+                         | None => True
+                       end |]%Sep).
+  destruct (NPure lhs).
+  apply SubstsH_inj_fwd.
+  apply SubstsH_emp_fwd.
+  apply Himp_star_pure_c; intro.
+  assert (SubstsH S
+    (fold_left (fun (hp : hpropB G) (p : pred) => predD p hE fE' * hp) x Emp) ===>
+    SubstsH S
+    (addQuants (NQuants rhs)
+      (fun fE0 : fo_env =>
+        fold_left (fun (hp : hpropB G) (p : pred) => predD p hE fE0 * hp)
+        (NImpure rhs)
+        Emp) fE)).
+  2: admit.
+
+  Lemma sub_expr_agrees : forall fE fE' s,
+    (forall x v, s x = Some v -> fE x = exprD v fE')
+    -> forall e e', sub_expr s e = Some e'
+      -> (forall fE fE',
+        (forall x, s x <> None -> fE x = fE' x)
+        -> exprD e fE = exprD e fE')
+      -> exprD e' fE' = exprD e fE.
   Proof.
     destruct e; simpl; intuition.
-    exfalso.
-    specialize (H (fun _ => Dyn tt) (fun _ => Dyn false)).
-    assert (forall x y : unit, x = y).
-    destruct x0, y; auto.
-    simpl in *.
-    apply (f_equal Ty) in H; simpl in *.
-    rewrite H in H1.
-    specialize (H1 true false); discriminate.
+    erewrite H; eauto.
+    injection H0; clear H0; intros; subst.
+    simpl.
+    apply H1.
+    intros.
+    specialize (H x).
+    destruct (s x); intuition.
+    symmetry; auto.
   Qed.
 
-  Lemma sub_pred_closed : forall s p,
-    wellScoped nil p
-    -> forall p', sub_pred s p = Some p'
-      -> p' = p.
+  Lemma sub_exprs_agrees : forall fE fE' s,
+    (forall x v, s x = Some v -> fE x = exprD v fE')
+    -> forall es es', (forall fE fE',
+      (forall x, s x <> None -> fE x = fE' x)
+      -> forall e, In e es -> exprD e fE = exprD e fE')
+    -> sub_exprs s es = Some es'
+    -> map (fun e => exprD e fE') es' = map (fun e => exprD e fE) es.
   Proof.
-    destruct p; simpl; intuition.
-    case_eq (sub_exprs s es); intros.
-    Focus 2.
-    rewrite H1 in H0; discriminate.
-    rewrite H1 in H0; injection H0; clear H0; intros; subst.
-    f_equal.
-    generalize dependent l.
-    induction es; simpl; intuition.
-    simpl in *.
-    case_eq (sub_expr s a); intros.
-    Focus 2.
-    rewrite H0 in *; discriminate.
-    rewrite H0 in *.
-    apply sub_expr_closed in H0; eauto.
-    subst.
-    case_eq (sub_exprs s es); intros.
-    Focus 2.
-    rewrite H0 in *; discriminate.
-    rewrite H0 in *.
+    induction es; simpl; intuition idtac.
+
     injection H1; clear H1; intros; subst.
-    f_equal; eauto.
-    intros; eapply H; auto; tauto.
-  Qed.
+    auto.
 
-  Lemma sub_preds_closed : forall s ps,
-    List.Forall (wellScoped nil) ps
-    -> forall ps', sub_preds s ps = Some ps'
-      -> ps' = ps.
-  Proof.
-    induction 1; simpl; intuition.
-    case_eq (sub_pred s x); intros.
+    case_eq (sub_expr s a); intros.
     Focus 2.
     rewrite H2 in *; discriminate.
     rewrite H2 in *.
-    case_eq (sub_preds s l); intros.
+    case_eq (sub_exprs s es); intros.
     Focus 2.
     rewrite H3 in *; discriminate.
     rewrite H3 in *.
-    injection H1; clear H1; intros; subst.
-    f_equal; auto.
-    eapply sub_pred_closed; eauto.
+    injection H1; clear H1; intros; subst; simpl in *.
+    f_equal.
+    eapply sub_expr_agrees; eauto.
+    eauto.
   Qed.
 
-  Lemma choose_existentials_expr : forall qs fE fE' s e e',
-    (forall fE fE', (forall x, In x qs -> fE x = fE' x)
-      -> exprD e fE = exprD e fE')
-    -> List.Forall (fun x => exists e, s x = Some e /\ fE x = exprD e fE') qs
-    -> sub_expr s e = Some e'
-    -> exprD e fE' = exprD e' fE.
+  Lemma sub_pred_agrees : forall G (hE : ho_env G) S fE fE' qs' s,
+    (forall x v, s x = Some v -> fE x = exprD v fE')
+    -> List.Forall (fun x => s x <> None)%type qs'
+    -> forall p p', wellScoped qs' p
+      -> sub_pred s p = Some p'
+      -> SubstsH S (predD p' hE fE') ===> SubstsH S (predD p hE fE).
   Proof.
-    destruct e; simpl; intuition.
-    Focus 2.
-    injection H1; clear H1; intros; subst.
-    simpl.
-    apply H.
-    intros.
-    eapply Forall_forall in H0; eauto.
-    
+    induction p; simpl; intuition.
 
-  Lemma choose_existentials_exprs : forall qs fE fE' s es es',
-    (forall fE fE', (forall x, In x qs -> fE x = fE' x)
-      -> forall e, In e es -> exprD e fE = exprD e fE')
-    -> List.Forall (fun x => exists e, s x = Some e /\ fE x = exprD e fE') qs
-    -> sub_exprs s es = Some es'
-    -> map (fun e => exprD e fE') es = map (fun e : expr => exprD e fE) es'.
-  Proof.
-    induction es; simpl; intuition.
-
-    injection H1; clear H1; intros; subst; auto.
-
-    case_eq (sub_e
-
-  Lemma choose_existentials_pred : forall G (hE : ho_env G) S qs p p' fE fE' s,
-     wellScoped qs p
-     -> List.Forall (fun x => exists e, s x = Some e /\ fE x = exprD e fE') qs
-     -> sub_pred s p = Some p'
-     -> SubstsH S (predD p hE fE') ===> SubstsH S (predD p' hE fE).
-  Proof.
-    destruct p; simpl; intuition.
     case_eq (sub_exprs s es); intros.
     Focus 2.
-    rewrite H2 in *; discriminate.
-    rewrite H2 in *.
-    injection H1; clear H1; intros; subst.
-    simpl.
-    
-
-
-  Lemma choose_existentials : forall G (hE : ho_env G) fE S s ps' qs qs' ps fE',
-    sub_preds s ps = Some ps'
-    -> List.Forall (wellScoped (qs ++ qs')) ps
-    -> List.Forall (fun x => exists e, s x = Some e /\ fE x = exprD e fE') qs'
-    -> SubstsH S (fold_left (fun hp p => predD p hE fE' * hp) ps' Emp)
-    ===> SubstsH S (addQuants qs
-      (fun fE0 => fold_left (fun hp p => predD p hE fE0 * hp) ps Emp) fE).
-  Proof.
-    induction qs; simpl; intuition.
-
-    generalize dependent ps'.
-    induction H0; simpl; intuition.
-    injection H; clear H; intros; subst.
-    apply Himp_refl.
-    case_eq (sub_pred s x); intros.
-    Focus 2.
-    rewrite H3 in H2; discriminate.
+    rewrite H3 in *; discriminate.
     rewrite H3 in *.
-    case_eq (sub_preds s l); intros.
+    injection H2; clear H2; intros; subst; simpl.
+    erewrite sub_exprs_agrees; try apply Himp_refl; eauto.
+    intros.
+    apply H1; eauto.
+    intros.
+    eapply Forall_forall in H0; eauto.
+  Qed.
+
+  Lemma sub_preds_agrees : forall G (hE : ho_env G) S fE fE' qs' s,
+    (forall x v, s x = Some v -> fE x = exprD v fE')
+    -> List.Forall (fun x => s x <> None)%type qs'
+    -> forall ps, List.Forall (wellScoped qs') ps
+      -> forall ps', sub_preds s ps = Some ps'
+        -> SubstsH S (fold_left (fun hp p => predD p hE fE' * hp) ps' Emp)
+        ===> SubstsH S (fold_left (fun hp p => predD p hE fE * hp) ps Emp).
+  Proof.
+    induction 3; simpl; intuition.
+
+    injection H1; clear H1; intros; subst.
+    apply Himp_refl.
+
+    eapply Himp_trans; [ | apply star_out_bwd ].
+    eapply Himp_trans; [ | apply SubstsH_star_bwd ].
+    case_eq (sub_pred s x); intros.
     Focus 2.
     rewrite H4 in *; discriminate.
     rewrite H4 in *.
-    injection H2; clear H2; intros; subst.
-    simpl.
+    case_eq (sub_preds s l); intros.
+    Focus 2.
+    rewrite H5 in *; discriminate.
+    rewrite H5 in *.
+    injection H3; clear H3; intros; subst; simpl.
     eapply Himp_trans; [ apply star_out_fwd | ].
     eapply Himp_trans; [ apply SubstsH_star_fwd | ].
-    eapply Himp_trans; [ | apply star_out_bwd ].
-    eapply Himp_trans; [ | apply SubstsH_star_bwd ].
     apply Himp_star_frame; auto.
+    eauto using sub_pred_agrees.
+  Qed.
 
-
-
-    replace ps' with ps.
-    admit. (*apply Himp_refl.*)
-    symmetry; eapply sub_preds_closed; eauto.
-
-    eapply Himp_trans; [ | apply SubstsH_ex_bwd ].
-    case_eq (s a); intros.
-    2: solve [ exfalso; eauto ].
-    apply Himp_ex_c; exists (exprD e fE).
-    apply IHqs.
-
-
-    
-
-    
-
-  Lemma choose_existentials : forall G (hE : ho_env G) fE S s rhs ps,
-    sub_preds s (NImpure rhs) = Some ps
-    -> match NPure rhs with
-         | None => True
-         | Some P => P fE
-       end
-    -> (forall x T, In (x, T) (NQuants rhs) -> s x <> None)
-    -> SubstsH S (fold_left (fun hp p => predD p hE fE * hp) ps Emp)
-    ===> SubstsH S (normalD rhs hE fE).
+  Lemma choose_existentials : forall G (hE : ho_env G) S s ps' ps,
+    sub_preds s ps = Some ps'
+    -> forall qs, List.Forall (fun x => s x <> None)%type qs
+      -> forall qs' fE fE', List.Forall (fun x => s x <> None)%type qs'
+        -> (forall x v, s x = Some v -> fE x = exprD v fE' \/ In x qs)
+        -> List.Forall (wellScoped (qs' ++ qs)) ps
+        -> SubstsH S (fold_left (fun hp p => predD p hE fE' * hp) ps' Emp)
+        ===> SubstsH S (addQuants qs
+          (fun fE0 => fold_left (fun hp p => predD p hE fE0 * hp) ps Emp) fE).
   Proof.
-    unfold normalD.
-    
-  
-  specialize (f
+    induction 2; simpl; intuition.
 
-  SearchAbout Himp empB.
-  apply Himp_emp.
-  SearchAbout fold_left SubstsH.
+    rewrite <- app_nil_end in *.
+    eapply sub_preds_agrees; eauto.
+    firstorder.
+
+    eapply Himp_trans; [ | eapply SubstsH_ex_bwd ].
+    apply Himp_ex_c.
+    case_eq (s x); intuition idtac.
+    exists (exprD e fE').
+    rewrite <- DepList.pf_list_simpl in H4.
+    eapply IHForall; try apply H4.
+    eauto using Forall_app.
+    intros.
+    destruct (string_dec x x0); subst.
+    rewrite H6 in H5; injection H5; clear H5; intros; subst.
+    autorewrite with core; auto.
+    autorewrite with core; auto.
+    specialize (H3 _ _ H6); tauto.
+  Qed.
+
+  eapply choose_existentials; eauto.
+  eapply Forall_forall; eauto.
+  intros.
+
+  Definition dyn1 := Dyn tt.
+  Definition dyn2 := Dyn false.
+
+  Theorem dyn_disc : dyn1 <> dyn2.
+  Proof.
+    intro.
+    apply (f_equal Ty) in H.
+    simpl in H.
+    assert (exists x : unit, forall y, x = y).
+    exists tt; destruct y; auto.
+    rewrite H in H0.
+    destruct H0.
+    specialize (H0 (negb x)).
+    destruct x; discriminate.
+  Qed.
+
+  Lemma unify_expr_adds : forall xs s lhs rhs s' Ps,
+    unify_expr s lhs rhs = Some (s', Ps)
+    -> (forall fE fE', (forall x, In x xs -> fE x = fE' x)
+      -> exprD rhs fE = exprD rhs fE')
+      -> forall x, s' x <> None -> s x <> None \/ In x xs.
+  Proof.
+    destruct lhs, rhs; simpl; intuition idtac; try discriminate.
+
+    destruct (s x0).
+    destruct e; try discriminate.
+    destruct (string_dec x2 x); subst; try discriminate.
+    injection H; clear H; intros; subst; tauto.
+    injection H; clear H; intros; subst.
+    unfold fos_set in H1.
+    destruct (string_dec x1 x0); subst; intuition idtac.
+    specialize (H0 (fun _ => dyn1)
+      (fun x => if string_dec x x0 then dyn2 else dyn1)).
+    simpl in H0.
+    destruct (string_dec x0 x0); try tauto.
+    destruct (In_dec string_dec x0 xs); intuition idtac.
+    match type of H0 with
+      | ?P -> _ => assert P
+    end.
+    intros.
+    destruct (string_dec x1 x0); try congruence.
+    subst; tauto.
+    intuition idtac.
+    destruct (dyn_disc H2).
+
+    destruct (s x); try discriminate.
+    destruct e; try discriminate.
+    injection H; clear H; intros; subst; tauto.
+    injection H; clear H; intros; subst.
+    specialize (H0 (fun _ => dyn1)
+      (fun x0 => if string_dec x x0 then dyn2 else dyn1)).
+    simpl in H0.
+    unfold fos_set in H1.
+    destruct (string_dec x x); try tauto.
+    destruct (string_dec x0 x); subst; intuition idtac.
+    destruct (In_dec string_dec x xs); intuition idtac.
+    match type of H0 with
+      | ?P -> _ => assert P
+    end.
+    intros.
+    destruct (string_dec x x0); try congruence.
+    subst; tauto.
+    intuition idtac.
+    destruct (dyn_disc H2).
+    
+    injection H; clear H; intros; subst; tauto.
+  Qed.
+
+  Lemma unify_args_adds : forall xs lhs rhs s s' Ps,
+    unify_args s lhs rhs = Some (s', Ps)
+    -> (forall fE fE', (forall x, In x xs -> fE x = fE' x)
+      -> forall e, In e rhs -> exprD e fE = exprD e fE')
+      -> forall x, s' x <> None -> s x <> None \/ In x xs.
+  Proof.
+    induction lhs; destruct rhs; simpl; intuition idtac; try discriminate.
+
+    injection H; clear H; intros; subst; tauto.
+    
+    case_eq (unify_expr s a e); intros.
+    Focus 2.
+    rewrite H2 in *; discriminate.
+    rewrite H2 in *.
+    destruct p.
+    case_eq (unify_args f lhs rhs); intros.
+    Focus 2.
+    rewrite H3 in *; discriminate.
+    rewrite H3 in *.
+    destruct p.
+    injection H; clear H; intros; subst.
+    edestruct IHlhs; try apply H3; eauto.
+    edestruct unify_expr_adds; try apply H2; eauto.
+  Qed.
+
+  Lemma unify_pred_adds : forall xs rhs s,
+    wellScoped xs rhs
+    -> forall lhs s' Ps, unify_pred s lhs rhs = Some (s', Ps)
+      -> forall x, s' x <> None -> s x <> None \/ In x xs.
+  Proof.
+    destruct lhs, rhs; simpl in *; intuition idtac; try discriminate.
+    destruct (string_dec X X0); subst; try discriminate.
+    edestruct unify_args_adds; eauto.
+  Qed.    
+
+  Lemma findMatching_adds : forall xs rhs s,
+    wellScoped xs rhs
+    -> forall lhs s' lhs' Ps, findMatching s lhs rhs = Success1 s' lhs' Ps
+      -> forall x, s' x <> None -> s x <> None \/ In x xs.
+  Proof.
+    induction lhs; simpl; intuition idtac.
+
+    discriminate.
+
+    case_eq (unify_pred s a rhs); intros.
+    rewrite H2 in *.
+    destruct p.
+    injection H0; clear H0; intros; subst.
+    edestruct unify_pred_adds; eauto.
+
+    rewrite H2 in *.
+    case_eq (findMatching s lhs rhs); intros.
+    Focus 2.
+    rewrite H3 in *; discriminate.
+    rewrite H3 in *.
+    injection H0; clear H0; intros; subst.
+    eauto.
+  Qed.
+
+  Lemma findMatchings_adds : forall xs rhs,
+    List.Forall (wellScoped xs) rhs
+    -> forall lhs s s' lhs' Ps, findMatchings s lhs rhs = Success1 s' lhs' Ps
+      -> forall x, s' x <> None -> s x <> None \/ In x xs.
+  Proof.
+    induction 1; simpl; intuition idtac.
+
+    injection H; clear H; intros; subst; tauto.
+
+    case_eq (findMatching s lhs x); intros.
+    Focus 2.
+    rewrite H3 in *; discriminate.
+    rewrite H3 in *.
+    case_eq (findMatchings NewSub NewLhs l); intros.
+    Focus 2.
+    rewrite H4 in H1; discriminate.
+    rewrite H4 in H1.
+    injection H1; clear H1; intros; subst.
+    edestruct IHForall; eauto.
+    edestruct findMatching_adds; eauto.
+  Qed.
+
+  edestruct findMatchings_adds; eauto.
+  congruence.
+  tauto.
+Qed.
